initial support for exhale of predicates
Todo:
* Check.

viper-total-heaps/Simulation/KnownFolded.thy
@@ -1,10 +1,15 @@
 theory KnownFolded
-  imports TotalViperSemantics.TotalSemantics ViperBoogieAbsValueInst BoogieInterface
+  imports TotalViperSemantics.TotalSemantics TotalViperSemantics.TotalExtConsProps ViperBoogieAbsValueInst BoogieInterface
 begin
 
 
 record knownfolded_rel_options =
   kf_turned_on :: bool
+  \<comment>\<open>Tracks the permission-guarded known-folded relation \<open>heap_knownfolded_rel_pos\<close> (defined below).
+     Unlike \<open>kf_turned_on\<close>, this flag can stay on during an exhale: the guarded relation is preserved
+     by every exhale step, whereas the unguarded one is invalidated as soon as a predicate loses all
+     of its permission.\<close>
+  kf_pos_turned_on :: bool
 
 
 context begin
@@ -162,6 +167,205 @@ next
 qed
 
 
+lemma pred_folds_perm_contains_heap_loc:
+  assumes "pred_folds_perm lp l nm"
+  shows "contains_heap_loc l nm"
+  using assms
+  by (induction rule: pred_folds_perm.inducts) (auto intro: contains_heap_loc.ContainsLocNested)
+
+
+lemma has_sumA_zero_nonneg_point:
+  fixes pf :: "'b \<Rightarrow> real"
+  assumes "pf has_sumA 0"
+      and "\<And>x. pf x \<ge> 0"
+    shows "pf y = 0"
+proof -
+  have "(pf has_sum pf y) {y}"
+    using has_sum_finite[of "{y}" pf]
+    by simp
+  hence "pf y \<le> 0"
+    using has_sum_mono_neutral[OF _ assms(1)] assms(2)
+    by fastforce
+  thus ?thesis
+    using assms(2)
+    by (simp add: order_antisym)
+qed
+
+
+text \<open>A known-folded witness inside a nested mask forces the permission sum of the
+      corresponding heap location to be non-zero. Note that no assumption on the permission
+      of the enclosing predicate is required, since \<^const>\<open>nm_loc_sum'\<close> recurses into a
+      sub-mask without rescaling it.\<close>
+
+lemma contains_heap_loc_not_nm_loc_sum_zero:
+  assumes "contains_heap_loc l nm"
+  shows "\<not> nm_loc_sum l nm 0"
+  using assms
+proof (induction rule: contains_heap_loc.inducts)
+  case (ContainsLocDirect nm)
+  show ?case
+  proof
+    assume "nm_loc_sum l nm 0"
+    hence "get_mh_nm nm l \<le> 0"
+      using mh_le_nm_loc_sum
+      by blast
+    thus False
+      using ContainsLocDirect
+      by simp
+  qed
+next
+  case (ContainsLocNested nm lp p nm_sub)
+  show ?case
+  proof
+    assume Sum: "nm_loc_sum l nm 0"
+    obtain mh fnm where "nm = NM mh fnm"
+      using nm_get_eq
+      by blast
+    from Sum[unfolded \<open>nm = _\<close>] obtain pf where
+      MhLe: "Rep_preal (mh l) \<le> Rep_preal (0 :: preal)" and
+      PfSum: "pf has_sumA (Rep_preal (0 :: preal) - Rep_preal (mh l))" and
+      Pf: "\<And>lp'. option_fold (\<lambda>lpm. nm_loc_sum' l (snd lpm) (pf lp')) (pf lp' = 0) (fnm lp')"
+      by auto
+
+    have PfNonneg: "\<And>lp'. pf lp' \<ge> 0"
+    proof -
+      fix lp'
+      show "pf lp' \<ge> 0"
+        apply (cases "fnm lp'")
+        using Pf[of lp'] apply simp
+        using Pf[of lp'] nm_loc_sum'_nonneg by fastforce
+    qed
+
+    have "Rep_preal (mh l) = 0"
+      by (metis MhLe order_antisym prat_non_negative zero_preal.rep_eq)
+    hence "pf has_sumA 0"
+      using PfSum
+      by (simp add: zero_preal.rep_eq)
+    hence "pf lp = 0"
+      by (rule has_sumA_zero_nonneg_point[OF _ PfNonneg])
+
+    moreover have "fnm lp = Some (p, nm_sub)"
+      using ContainsLocNested.hyps(1) \<open>nm = _\<close>
+      by simp
+
+    ultimately have "nm_loc_sum l nm_sub 0"
+      using Pf[of lp]
+      by (simp add: zero_preal.rep_eq)
+
+    thus False
+      using ContainsLocNested.IH
+      by blast
+  qed
+qed
+
+
+lemma consistent_external_wrt_ploc_same_support:
+  assumes "consistent_external_wrt_ploc ctxt (\<phi>\<lparr> get_nm_total := nm\<^sub>1 \<rparr>) lp q\<^sub>1"
+      and "consistent_external_wrt_ploc ctxt (\<phi>\<lparr> get_nm_total := nm\<^sub>2 \<rparr>) lp q\<^sub>2"
+      and "q\<^sub>1 > 0" and "q\<^sub>2 > 0"
+    shows "(\<forall>l. (0 < get_mh_nm nm\<^sub>1 l) = (0 < get_mh_nm nm\<^sub>2 l)) \<and>
+           (\<forall>lp. (0 < get_mp_nm nm\<^sub>1 lp) = (0 < get_mp_nm nm\<^sub>2 lp))"
+proof -
+  obtain pid vs where "lp = (pid, vs)"
+    by fastforce
+  obtain pdecl\<^sub>1 pbody\<^sub>1 where
+    D\<^sub>1: "ViperLang.predicates (program_total ctxt) pid = Some pdecl\<^sub>1"
+        "ViperLang.predicate_decl.body pdecl\<^sub>1 = Some pbody\<^sub>1" and
+    Sat\<^sub>1: "sat ctxt \<lparr> get_store_total = nth_option vs, get_trace_total = Map.empty,
+                     get_total_full = \<phi>\<lparr> get_nm_total := 0 \<rparr> \<rparr>
+              (get_mh_nm nm\<^sub>1) (get_mp_nm nm\<^sub>1) (syntactic_mult (Rep_preal q\<^sub>1) pbody\<^sub>1)"
+    using assms(1)[unfolded \<open>lp = _\<close>] assms(3)
+    by (auto elim: SatStep_case)
+  obtain pdecl\<^sub>2 pbody\<^sub>2 where
+    D\<^sub>2: "ViperLang.predicates (program_total ctxt) pid = Some pdecl\<^sub>2"
+        "ViperLang.predicate_decl.body pdecl\<^sub>2 = Some pbody\<^sub>2" and
+    Sat\<^sub>2: "sat ctxt \<lparr> get_store_total = nth_option vs, get_trace_total = Map.empty,
+                     get_total_full = \<phi>\<lparr> get_nm_total := 0 \<rparr> \<rparr>
+              (get_mh_nm nm\<^sub>2) (get_mp_nm nm\<^sub>2) (syntactic_mult (Rep_preal q\<^sub>2) pbody\<^sub>2)"
+    using assms(2)[unfolded \<open>lp = _\<close>] assms(4)
+    by (auto elim: SatStep_case)
+  have "pbody\<^sub>1 = pbody\<^sub>2"
+    using D\<^sub>1 D\<^sub>2
+    by simp
+  moreover have "Rep_preal q\<^sub>1 > 0" and "Rep_preal q\<^sub>2 > 0"
+    using assms(3,4)
+    by (simp_all add: less_preal.rep_eq zero_preal.rep_eq)
+  ultimately show ?thesis
+    using sat_same_support[OF Sat\<^sub>1] Sat\<^sub>2
+    by simp
+qed
+
+
+text \<open>Two copies of the same predicate instance in a state have the same footprint: external
+      consistency forces both sub-masks to satisfy the same (scaled) predicate body, evaluated in
+      the same state, and by \<^const>\<open>sat\<close> the support of a satisfying mask does not depend on the
+      scaling factor. Consequently a location that lies under one copy also lies under the other.\<close>
+
+lemma contains_heap_loc_transfer:
+  assumes "contains_heap_loc l nm\<^sub>1"
+      and "consistent_external_wrt_ploc ctxt (\<phi>\<lparr> get_nm_total := nm\<^sub>1 \<rparr>) lp q\<^sub>1"
+      and "consistent_external_wrt_ploc ctxt (\<phi>\<lparr> get_nm_total := nm\<^sub>2 \<rparr>) lp q\<^sub>2"
+      and "q\<^sub>1 > 0" and "q\<^sub>2 > 0"
+    shows "contains_heap_loc l nm\<^sub>2"
+  using assms
+proof (induct arbitrary: nm\<^sub>2 lp q\<^sub>1 q\<^sub>2 rule: contains_heap_loc.inducts)
+  case (ContainsLocDirect nm\<^sub>1)
+  show ?case
+    apply (rule contains_heap_loc.ContainsLocDirect)
+    using consistent_external_wrt_ploc_same_support
+            [OF ContainsLocDirect.prems(1,2,3,4)] ContainsLocDirect.hyps
+    by blast
+next
+  case (ContainsLocNested nm\<^sub>1 lp' p' nm')
+  note Support = consistent_external_wrt_ploc_same_support[OF ContainsLocNested.prems(1,2,3,4)]
+
+  have MpPos\<^sub>1: "0 < get_mp_nm nm\<^sub>1 lp'"
+    using ContainsLocNested.hyps(1) Rep_posreal
+    by simp
+  hence "0 < get_mp_nm nm\<^sub>2 lp'"
+    using Support
+    by blast
+  from this obtain p'' nm'' where Slot\<^sub>2: "get_fnm_nm nm\<^sub>2 lp' = Some (p'', nm'')"
+    by (cases "get_fnm_nm nm\<^sub>2 lp'") auto
+
+  obtain pid vs where "lp = (pid, vs)"
+    by fastforce
+  obtain pid' vs' where "lp' = (pid', vs')"
+    by fastforce
+
+  have Cons\<^sub>1: "consistent_external ctxt (\<phi>\<lparr> get_nm_total := nm\<^sub>1 \<rparr>)"
+    using ContainsLocNested.prems(1)[unfolded \<open>lp = _\<close>]
+    by (auto elim: SatStep_case)
+  have Cons\<^sub>2: "consistent_external ctxt (\<phi>\<lparr> get_nm_total := nm\<^sub>2 \<rparr>)"
+    using ContainsLocNested.prems(2)[unfolded \<open>lp = _\<close>]
+    by (auto elim: SatStep_case)
+
+  have All\<^sub>1: "\<And>pid\<^sub>0 vs\<^sub>0 q\<^sub>0 nm\<^sub>0. Some (q\<^sub>0, nm\<^sub>0) = get_fnm_nm nm\<^sub>1 (pid\<^sub>0, vs\<^sub>0) \<Longrightarrow>
+        consistent_external_wrt_ploc ctxt (\<phi>\<lparr> get_nm_total := nm\<^sub>0 \<rparr>) (pid\<^sub>0, vs\<^sub>0) (Rep_posreal q\<^sub>0)"
+    using Cons\<^sub>1
+    by (auto elim: SatAll_case)
+  have All\<^sub>2: "\<And>pid\<^sub>0 vs\<^sub>0 q\<^sub>0 nm\<^sub>0. Some (q\<^sub>0, nm\<^sub>0) = get_fnm_nm nm\<^sub>2 (pid\<^sub>0, vs\<^sub>0) \<Longrightarrow>
+        consistent_external_wrt_ploc ctxt (\<phi>\<lparr> get_nm_total := nm\<^sub>0 \<rparr>) (pid\<^sub>0, vs\<^sub>0) (Rep_posreal q\<^sub>0)"
+    using Cons\<^sub>2
+    by (auto elim: SatAll_case)
+
+  have Sub\<^sub>1: "consistent_external_wrt_ploc ctxt (\<phi>\<lparr> get_nm_total := nm' \<rparr>) lp' (Rep_posreal p')"
+    using All\<^sub>1 ContainsLocNested.hyps(1) \<open>lp' = _\<close>
+    by fastforce
+  have Sub\<^sub>2: "consistent_external_wrt_ploc ctxt (\<phi>\<lparr> get_nm_total := nm'' \<rparr>) lp' (Rep_posreal p'')"
+    using All\<^sub>2 Slot\<^sub>2 \<open>lp' = _\<close>
+    by fastforce
+
+  have "contains_heap_loc l nm''"
+    apply (rule ContainsLocNested.hyps(3)[OF Sub\<^sub>1 Sub\<^sub>2])
+    using Rep_posreal
+    by simp_all
+
+  thus ?case
+    by (rule contains_heap_loc.ContainsLocNested[OF Slot\<^sub>2])
+qed
+
+
 definition heap_knownfolded_rel :: "ViperLang.program \<Rightarrow> (field_ident \<rightharpoonup> vname) \<Rightarrow> 'a nested_mask \<Rightarrow> 'a bpl_heap_ty \<Rightarrow> bool"
   where "heap_knownfolded_rel Pr tr_field nm hb \<equiv>
     \<forall>lp kfm l field_ty_vpr field_bpl.
@@ -172,12 +376,327 @@ definition heap_knownfolded_rel :: "ViperLang.program \<Rightarrow> (field_ident
         pred_folds_perm lp l nm"
 
 
+text \<open>Permission-guarded variant of \<^const>\<open>heap_knownfolded_rel\<close>: the known-folded mask stored in
+      the Boogie heap must only be backed by real permission for those predicate locations that
+      still hold permission. This is the property that the \<open>IdenticalOnKnownLocations\<close> axioms
+      require (they are guarded by \<open>Mask[null, pm_f] > 0\<close>), and unlike \<^const>\<open>heap_knownfolded_rel\<close>
+      it survives an exhale that removes all permission of a predicate.\<close>
+
+definition heap_knownfolded_rel_pos :: "ViperLang.program \<Rightarrow> (field_ident \<rightharpoonup> vname) \<Rightarrow> 'a nested_mask \<Rightarrow> 'a bpl_heap_ty \<Rightarrow> bool"
+  where "heap_knownfolded_rel_pos Pr tr_field nm hb \<equiv>
+    \<forall>lp kfm l field_ty_vpr field_bpl.
+        get_mp_nm nm lp > 0 \<longrightarrow>
+        hb (Null, PredKnownFoldedField lp) = Some (AbsV (AKnownFoldedMask kfm)) \<longrightarrow>
+        declared_fields Pr (snd l) = Some field_ty_vpr \<longrightarrow>
+        tr_field (snd l) = Some field_bpl \<longrightarrow>
+        kfm (Address (fst l), NormalField field_bpl field_ty_vpr) \<longrightarrow>
+        pred_folds_perm lp l nm"
+
+
+lemma heap_knownfolded_rel_pos_stable:
+  assumes "heap_knownfolded_rel_pos Pr tr_field nm hb"
+      and "\<And>lp. hb' (Null, PredKnownFoldedField lp) = hb (Null, PredKnownFoldedField lp)"
+    shows "heap_knownfolded_rel_pos Pr tr_field nm hb'"
+  using assms
+  unfolding heap_knownfolded_rel_pos_def
+  by simp
+
+
+lemma heap_knownfolded_rel_imp_pos:
+  assumes "heap_knownfolded_rel Pr tr_field nm hb"
+  shows "heap_knownfolded_rel_pos Pr tr_field nm hb"
+  using assms
+  unfolding heap_knownfolded_rel_def heap_knownfolded_rel_pos_def
+  by blast
+
+
+text \<open>The known-folded masks stored in the Boogie heap only ever flag normal field locations. This
+      holds independently of whether the known-folded relation is currently tracked, and is required
+      when the exhale havoc resets the known-folded mask of a predicate without permission: without
+      it, a known-folded mask could refer to another predicate's known-folded mask location, which
+      the framing axioms would then force to be preserved.\<close>
+
+definition knownfolded_masks_normal_fields :: "'a bpl_heap_ty \<Rightarrow> bool"
+  where "knownfolded_masks_normal_fields hb \<equiv>
+    \<forall>lp kfm r f. hb (Null, PredKnownFoldedField lp) = Some (AbsV (AKnownFoldedMask kfm)) \<longrightarrow>
+                 kfm (r, f) \<longrightarrow> is_NormalField f"
+
+
+text \<open>A witness for a predicate that holds top-level permission can always be found in that
+      predicate's own sub-mask.\<close>
+
+lemma pred_folds_perm_direct_witness_aux:
+  assumes "pred_folds_perm lp l nm"
+      and "consistent_external ctxt (\<phi>\<lparr> get_nm_total := nm \<rparr>)"
+      and "consistent_external_wrt_ploc ctxt (\<phi>\<lparr> get_nm_total := nm_sub \<rparr>) lp q"
+      and "q > 0"
+    shows "contains_heap_loc l nm_sub"
+  using assms
+proof (induct rule: pred_folds_perm.inducts)
+  case (ContainsPermDirect nm q' nm')
+  have All: "\<And>pid\<^sub>0 vs\<^sub>0 q\<^sub>0 nm\<^sub>0. Some (q\<^sub>0, nm\<^sub>0) = get_fnm_nm nm (pid\<^sub>0, vs\<^sub>0) \<Longrightarrow>
+        consistent_external_wrt_ploc ctxt (\<phi>\<lparr> get_nm_total := nm\<^sub>0 \<rparr>) (pid\<^sub>0, vs\<^sub>0) (Rep_posreal q\<^sub>0)"
+    using ContainsPermDirect.prems(1)
+    by (auto elim: SatAll_case)
+  obtain pid vs where "lp = (pid, vs)"
+    by fastforce
+  have "consistent_external_wrt_ploc ctxt (\<phi>\<lparr> get_nm_total := nm' \<rparr>) lp (Rep_posreal q')"
+    using All ContainsPermDirect.hyps(1) \<open>lp = _\<close>
+    by fastforce
+  thus ?case
+    using contains_heap_loc_transfer[OF ContainsPermDirect.hyps(2) _ ContainsPermDirect.prems(2)]
+          ContainsPermDirect.prems(3) Rep_posreal
+    by simp
+next
+  case (ContainsPermNested nm lp'' q'' nm'')
+  have All: "\<And>pid\<^sub>0 vs\<^sub>0 q\<^sub>0 nm\<^sub>0. Some (q\<^sub>0, nm\<^sub>0) = get_fnm_nm nm (pid\<^sub>0, vs\<^sub>0) \<Longrightarrow>
+        consistent_external_wrt_ploc ctxt (\<phi>\<lparr> get_nm_total := nm\<^sub>0 \<rparr>) (pid\<^sub>0, vs\<^sub>0) (Rep_posreal q\<^sub>0)"
+    using ContainsPermNested.prems(1)
+    by (auto elim: SatAll_case)
+  obtain pid'' vs'' where "lp'' = (pid'', vs'')"
+    by fastforce
+  have "consistent_external_wrt_ploc ctxt (\<phi>\<lparr> get_nm_total := nm'' \<rparr>) lp'' (Rep_posreal q'')"
+    using All ContainsPermNested.hyps(1) \<open>lp'' = _\<close>
+    by fastforce
+  hence "consistent_external ctxt (\<phi>\<lparr> get_nm_total := nm'' \<rparr>)"
+    using \<open>lp'' = _\<close>
+    by (auto elim: SatStep_case)
+  thus ?case
+    using ContainsPermNested.hyps(3) ContainsPermNested.prems(2,3)
+    by blast
+qed
+
+
+lemma pred_folds_perm_direct_witness:
+  assumes "pred_folds_perm lp l (get_nm_total \<phi>)"
+      and "consistent_external ctxt \<phi>"
+      and "get_fnm_total \<phi> lp = Some (q, nm_sub)"
+    shows "contains_heap_loc l nm_sub"
+proof -
+  have All: "\<And>pid\<^sub>0 vs\<^sub>0 q\<^sub>0 nm\<^sub>0. Some (q\<^sub>0, nm\<^sub>0) = get_fnm_total \<phi> (pid\<^sub>0, vs\<^sub>0) \<Longrightarrow>
+        consistent_external_wrt_ploc ctxt (\<phi>\<lparr> get_nm_total := nm\<^sub>0 \<rparr>) (pid\<^sub>0, vs\<^sub>0) (Rep_posreal q\<^sub>0)"
+    using assms(2)
+    by (auto elim: SatAll_case)
+  obtain pid vs where "lp = (pid, vs)"
+    by fastforce
+  have Sub: "consistent_external_wrt_ploc ctxt (\<phi>\<lparr> get_nm_total := nm_sub \<rparr>) lp (Rep_posreal q)"
+    using All assms(3) \<open>lp = _\<close>
+    by fastforce
+  have Eq: "\<phi>\<lparr> get_nm_total := get_nm_total \<phi> \<rparr> = \<phi>"
+    by simp
+  show ?thesis
+    apply (rule pred_folds_perm_direct_witness_aux[OF assms(1) _ Sub])
+    using assms(2) Eq
+     apply simp
+    using Rep_posreal
+    by simp
+qed
+
+
+text \<open>Preservation of the permission-guarded known-folded relation by the two state updates an
+      exhale can perform. Exhaling a field access only changes the top-level field mask, which
+      \<^const>\<open>pred_folds_perm\<close> does not depend on. Exhaling a predicate access either scales that
+      predicate's sub-mask by a positive factor or removes its slot altogether, in which case the
+      permission guard no longer applies to it; for all other predicates the slot is untouched, and
+      a witness in the predicate's own slot is available by \<open>pred_folds_perm_direct_witness\<close>.\<close>
+
+lemma heap_knownfolded_rel_pos_fnm_stable:
+  assumes "heap_knownfolded_rel_pos Pr tr_field nm hb"
+      and "get_fnm_nm nm = get_fnm_nm nm'"
+    shows "heap_knownfolded_rel_pos Pr tr_field nm' hb"
+  unfolding heap_knownfolded_rel_pos_def
+proof (intro allI impI)
+  fix lp kfm l field_ty_vpr field_bpl
+  assume "0 < get_mp_nm nm' lp"
+     and "hb (Null, PredKnownFoldedField lp) = Some (AbsV (AKnownFoldedMask kfm))"
+     and "declared_fields Pr (snd l) = Some field_ty_vpr"
+     and "tr_field (snd l) = Some field_bpl"
+     and "kfm (Address (fst l), NormalField field_bpl field_ty_vpr)"
+  moreover have "\<And>lp\<^sub>0. get_mp_nm nm' lp\<^sub>0 = get_mp_nm nm lp\<^sub>0"
+    using assms(2)
+    by simp
+  ultimately have "0 < get_mp_nm nm lp"
+    by metis
+  hence "pred_folds_perm lp l nm"
+    using assms(1) \<open>hb _ = _\<close> \<open>declared_fields _ _ = _\<close> \<open>tr_field _ = _\<close> \<open>kfm _\<close>
+    unfolding heap_knownfolded_rel_pos_def
+    by blast
+  thus "pred_folds_perm lp l nm'"
+    using pred_folds_perm_mh_stable assms(2)
+    by blast
+qed
+
+lemma heap_knownfolded_rel_pos_rm_from_lpm:
+  assumes "heap_knownfolded_rel_pos Pr tr_field (get_nm_total \<phi>) hb"
+      and "consistent_external ctxt \<phi>"
+    shows "heap_knownfolded_rel_pos Pr tr_field (rm_from_lpm_nm (get_nm_total \<phi>) lp\<^sub>0 p) hb"
+  unfolding heap_knownfolded_rel_pos_def
+proof (intro allI impI)
+  fix lp kfm l field_ty_vpr field_bpl
+  let ?nm = "get_nm_total \<phi>"
+  let ?nm' = "rm_from_lpm_nm ?nm lp\<^sub>0 p"
+  assume Guard: "0 < get_mp_nm ?nm' lp"
+     and Kfm: "hb (Null, PredKnownFoldedField lp) = Some (AbsV (AKnownFoldedMask kfm))"
+     and Decl: "declared_fields Pr (snd l) = Some field_ty_vpr"
+     and Tr: "tr_field (snd l) = Some field_bpl"
+     and Flag: "kfm (Address (fst l), NormalField field_bpl field_ty_vpr)"
+
+  have Other: "\<And>lp'. lp' \<noteq> lp\<^sub>0 \<Longrightarrow> get_fnm_nm ?nm' lp' = get_fnm_nm ?nm lp'"
+    by (cases ?nm) simp
+
+  show "pred_folds_perm lp l ?nm'"
+  proof (cases "lp = lp\<^sub>0")
+    case False
+    hence "get_mp_nm ?nm lp > 0"
+      using Guard Other
+      by simp
+    hence "pred_folds_perm lp l ?nm"
+      using assms(1) Kfm Decl Tr Flag
+      unfolding heap_knownfolded_rel_pos_def
+      by blast
+    moreover obtain q nm_sub where Slot: "get_fnm_total \<phi> lp = Some (q, nm_sub)"
+      using \<open>get_mp_nm ?nm lp > 0\<close>
+      by (cases "get_fnm_nm ?nm lp") auto
+    ultimately have "contains_heap_loc l nm_sub"
+      using pred_folds_perm_direct_witness[OF _ assms(2) Slot]
+      by simp
+    thus ?thesis
+      apply (rule pred_folds_perm.ContainsPermDirect[rotated])
+      using Slot Other False
+      by simp
+  next
+    case True
+    obtain q nm_sub where Slot: "get_fnm_nm ?nm lp\<^sub>0 = Some (q, nm_sub)" and
+                          NotRemoved: "\<not> (p \<ge> Rep_posreal q)"
+      using Guard True
+      by (cases "get_fnm_nm ?nm lp\<^sub>0"; cases ?nm) (auto split: if_split_asm)
+    have Slot': "get_fnm_nm ?nm' lp\<^sub>0 =
+                   Some (Abs_posreal (Rep_posreal q - p), (1 - p / Rep_posreal q) *\<^sub>s nm_sub)"
+      using Slot NotRemoved
+      by (cases ?nm) simp
+    have "get_mp_nm ?nm lp\<^sub>0 > 0"
+      using Slot Rep_posreal
+      by simp
+    hence "pred_folds_perm lp l ?nm"
+      using assms(1) Kfm Decl Tr Flag True
+      unfolding heap_knownfolded_rel_pos_def
+      by blast
+    hence Contains: "contains_heap_loc l nm_sub"
+      using pred_folds_perm_direct_witness[OF _ assms(2)] Slot True
+      by simp
+    have Pos: "(1 :: preal) - p / Rep_posreal q > 0"
+    proof -
+      have "Rep_preal (Rep_posreal q) > 0"
+        using Rep_posreal
+        by (simp add: less_preal.rep_eq zero_preal.rep_eq)
+      moreover have "Rep_preal p < Rep_preal (Rep_posreal q)"
+        using NotRemoved
+        by (simp add: less_eq_preal.rep_eq linorder_not_le less_preal.rep_eq)
+      ultimately show ?thesis
+        by (simp add: preal_to_real prat_non_negative)
+    qed
+    have Scaled: "contains_heap_loc l ((1 - p / Rep_posreal q) *\<^sub>s nm_sub)"
+      by (rule contains_heap_loc_scale[OF Contains Pos])
+    show ?thesis
+      apply (rule pred_folds_perm.ContainsPermDirect[rotated])
+       apply (rule Scaled)
+      using Slot' True
+      by simp
+  qed
+qed
+
+
 definition heap_knownfolded_var_rel :: "knownfolded_rel_options \<Rightarrow> ViperLang.program \<Rightarrow> var_context \<Rightarrow> (field_ident \<rightharpoonup> Lang.vname) \<Rightarrow> vname \<Rightarrow> 'a full_total_state \<Rightarrow> ('a vbpl_absval) nstate \<Rightarrow> bool"
   where
     "heap_knownfolded_var_rel opt Pr \<Lambda> FieldTr hvar \<omega> ns \<equiv> \<exists>hb.
        lookup_var \<Lambda> ns hvar = Some (AbsV (AHeap hb)) \<and>
        (\<forall>lp. \<exists>kfm. hb (Null, PredKnownFoldedField lp) = Some (AbsV (AKnownFoldedMask kfm))) \<and>
-       (kf_turned_on opt \<longrightarrow> heap_knownfolded_rel Pr FieldTr (get_nm_total_full \<omega>) hb)"
+       knownfolded_masks_normal_fields hb \<and>
+       (kf_turned_on opt \<longrightarrow> heap_knownfolded_rel Pr FieldTr (get_nm_total_full \<omega>) hb) \<and>
+       (kf_pos_turned_on opt \<longrightarrow> heap_knownfolded_rel_pos Pr FieldTr (get_nm_total_full \<omega>) hb)"
+
+
+lemma knownfolded_masks_normal_fields_elim:
+  assumes "knownfolded_masks_normal_fields hb"
+      and "hb (Null, PredKnownFoldedField lp) = Some (AbsV (AKnownFoldedMask kfm))"
+      and "kfm (r, f)"
+    shows "is_NormalField f"
+  using assms
+  unfolding knownfolded_masks_normal_fields_def
+  by blast
+
+
+lemma kfm_flag_upd_normal_field:
+  assumes "\<And>r f. kfm (r, f) \<Longrightarrow> is_NormalField f"
+      and "(kfm((r', NormalField fb ft) := True)) (r, f)"
+    shows "is_NormalField f"
+  using assms
+  by (auto split: if_split_asm)
+
+
+lemma knownfolded_masks_normal_fields_upd:
+  assumes "knownfolded_masks_normal_fields hb"
+      and "\<And>r f. kfm (r, f) \<Longrightarrow> is_NormalField f"
+    shows "knownfolded_masks_normal_fields (hb((Null, PredKnownFoldedField lp) \<mapsto> AbsV (AKnownFoldedMask kfm)))"
+  using assms
+  unfolding knownfolded_masks_normal_fields_def
+  by auto
+
+
+lemma heap_knownfolded_var_rel_masks_normal_fields:
+  assumes "heap_knownfolded_var_rel opt Pr \<Lambda> FieldTr hvar \<omega> ns"
+      and "lookup_var \<Lambda> ns hvar = Some (AbsV (AHeap hb))"
+    shows "knownfolded_masks_normal_fields hb"
+  using assms
+  unfolding heap_knownfolded_var_rel_def
+  by auto
+
+
+text \<open>Packaged form of the preservation lemmas for the state update performed when exhaling a
+      predicate access: the Boogie heap is unchanged, the unguarded relation is not tracked, and the
+      guarded one is preserved.\<close>
+
+lemma heap_knownfolded_var_rel_rm_from_lpm:
+  assumes "heap_knownfolded_var_rel opt Pr \<Lambda> FieldTr hvar \<omega> ns"
+      and "\<not> kf_turned_on opt"
+      and "kf_pos_turned_on opt \<Longrightarrow> consistent_external ctxt (get_total_full \<omega>)"
+      and "lookup_var \<Lambda> ns hvar = lookup_var \<Lambda> ns' hvar"
+      and "\<omega>' = rm_from_lpm_total_full \<omega> lp p"
+    shows "heap_knownfolded_var_rel opt Pr \<Lambda> FieldTr hvar \<omega>' ns'"
+proof -
+  obtain hb where hb:
+    "lookup_var \<Lambda> ns hvar = Some (AbsV (AHeap hb))"
+    "\<forall>lp. \<exists>kfm. hb (Null, PredKnownFoldedField lp) = Some (AbsV (AKnownFoldedMask kfm))"
+    "knownfolded_masks_normal_fields hb"
+    "kf_pos_turned_on opt \<longrightarrow> heap_knownfolded_rel_pos Pr FieldTr (get_nm_total_full \<omega>) hb"
+    using assms(1)
+    unfolding heap_knownfolded_var_rel_def
+    by blast
+
+  have Nm: "get_nm_total_full \<omega>' = rm_from_lpm_nm (get_nm_total (get_total_full \<omega>)) lp p"
+    using assms(5)
+    by simp
+
+  show ?thesis
+    unfolding heap_knownfolded_var_rel_def
+    apply (rule exI[of _ hb])
+    apply (intro conjI)
+    using hb(1) assms(4)
+       apply argo
+    using hb(2)
+      apply blast
+    using hb(3)
+     apply blast
+    using assms(2)
+     apply blast
+    apply (intro impI)
+    apply (simp only: Nm)
+    apply (rule heap_knownfolded_rel_pos_rm_from_lpm[where \<phi> = "get_total_full \<omega>"])
+    using hb(4)
+     apply simp
+    using assms(3)
+    by simp
+qed
 
 
 lemma heap_knownfolded_var_rel_stable:
@@ -198,7 +717,8 @@ lemma heap_knownfolded_var_rel_stable_kfm_unchanged:
       and "\<And>r lp. hb (r, PredKnownFoldedField lp) = hb' (r, PredKnownFoldedField lp)"
     shows "heap_knownfolded_var_rel opt Pr \<Lambda> FieldTr hvar \<omega> ns'"
   using assms
-  unfolding heap_knownfolded_var_rel_def heap_knownfolded_rel_def
+  unfolding heap_knownfolded_var_rel_def heap_knownfolded_rel_def heap_knownfolded_rel_pos_def
+            knownfolded_masks_normal_fields_def
   by auto
 
 
@@ -210,28 +730,52 @@ lemma heap_knownfolded_var_rel_stable_mh_changed:
 proof -
   obtain hb where hb: "lookup_var \<Lambda> ns hvar = Some (AbsV (AHeap hb)) \<and>
                        (\<forall>lp. \<exists>kfm. hb (Null, PredKnownFoldedField lp) = Some (AbsV (AKnownFoldedMask kfm))) \<and>
-                       (kf_turned_on opt \<longrightarrow> heap_knownfolded_rel Pr FieldTr (get_nm_total_full \<omega>) hb)"
+                       knownfolded_masks_normal_fields hb \<and>
+                       (kf_turned_on opt \<longrightarrow> heap_knownfolded_rel Pr FieldTr (get_nm_total_full \<omega>) hb) \<and>
+                       (kf_pos_turned_on opt \<longrightarrow> heap_knownfolded_rel_pos Pr FieldTr (get_nm_total_full \<omega>) hb)"
     using assms(1) heap_knownfolded_var_rel_def
     by blast
+
+  have GuardSame: "get_mp_nm (get_nm_total_full \<omega>') = get_mp_nm (get_nm_total_full \<omega>)"
+    using assms(2)
+    by simp
+
   show ?thesis
     unfolding heap_knownfolded_var_rel_def
     apply (rule exI[of _ hb])
     apply (intro conjI)
     using hb assms(3)
-      apply argo
+        apply argo
     using hb
-     apply blast
+       apply blast
+    using hb
+      apply blast
+     defer
   proof
-    assume "kf_turned_on opt"
-    hence *: "heap_knownfolded_rel Pr FieldTr (get_nm_total_full \<omega>) hb"
+    assume "kf_pos_turned_on opt"
+    hence *: "heap_knownfolded_rel_pos Pr FieldTr (get_nm_total_full \<omega>) hb"
       using hb
       by force
-    show "heap_knownfolded_rel Pr FieldTr (get_nm_total_full \<omega>') hb"
-      unfolding heap_knownfolded_rel_def
+    show "heap_knownfolded_rel_pos Pr FieldTr (get_nm_total_full \<omega>') hb"
+      unfolding heap_knownfolded_rel_pos_def
       apply (intro impI allI)
-      using * pred_folds_perm_mh_stable assms(2,3)
-      unfolding heap_knownfolded_rel_def
+      using * pred_folds_perm_mh_stable assms(2) GuardSame
+      unfolding heap_knownfolded_rel_pos_def
       by fastforce
+  next
+    show "kf_turned_on opt \<longrightarrow> heap_knownfolded_rel Pr FieldTr (get_nm_total_full \<omega>') hb"
+    proof
+      assume "kf_turned_on opt"
+      hence *: "heap_knownfolded_rel Pr FieldTr (get_nm_total_full \<omega>) hb"
+        using hb
+        by force
+      show "heap_knownfolded_rel Pr FieldTr (get_nm_total_full \<omega>') hb"
+        unfolding heap_knownfolded_rel_def
+        apply (intro impI allI)
+        using * pred_folds_perm_mh_stable assms(2,3)
+        unfolding heap_knownfolded_rel_def
+        by fastforce
+    qed
   qed
 qed
 
@@ -244,12 +788,49 @@ lemma heap_knownfolded_rel_stable_larger_nm:
   by (smt (verit, ccfv_threshold) assms heap_knownfolded_rel_def)
 
 
+text \<open>Growing the state can turn the permission guard on for further predicates, so the guarded
+      relation is not preserved on its own. It is preserved whenever the unguarded relation is
+      tracked as well, which is the case everywhere the state grows (the guarded relation is only
+      tracked on its own during an exhale, where the state never grows).\<close>
+
 lemma heap_knownfolded_var_rel_stable_larger_\<omega>:
   assumes "heap_knownfolded_var_rel opt Pr \<Lambda> FieldTr hvar \<omega> ns"
       and "\<omega> \<le> \<omega>'"
       and "lookup_var \<Lambda> ns hvar = lookup_var \<Lambda> ns' hvar"
+      and PosImpliesStrict: "kf_pos_turned_on opt \<Longrightarrow> kf_turned_on opt"
     shows "heap_knownfolded_var_rel opt Pr \<Lambda> FieldTr hvar \<omega>' ns'"
-  by (smt (verit, best) assms(1,2,3) heap_knownfolded_rel_stable_larger_nm heap_knownfolded_var_rel_def less_eq_full_total_stateD_2)
+proof -
+  obtain hb where hb:
+    "lookup_var \<Lambda> ns hvar = Some (AbsV (AHeap hb))"
+    "\<forall>lp. \<exists>kfm. hb (Null, PredKnownFoldedField lp) = Some (AbsV (AKnownFoldedMask kfm))"
+    "knownfolded_masks_normal_fields hb"
+    "kf_turned_on opt \<longrightarrow> heap_knownfolded_rel Pr FieldTr (get_nm_total_full \<omega>) hb"
+    using assms(1)
+    unfolding heap_knownfolded_var_rel_def
+    by blast
+
+  have Strict: "kf_turned_on opt \<longrightarrow> heap_knownfolded_rel Pr FieldTr (get_nm_total_full \<omega>') hb"
+    using hb(4) assms(2) heap_knownfolded_rel_stable_larger_nm less_eq_full_total_stateD_2
+    by blast
+
+  show ?thesis
+    unfolding heap_knownfolded_var_rel_def
+    apply (rule exI[of _ hb])
+    apply (intro conjI)
+    using hb(1) assms(3)
+       apply argo
+    using hb(2)
+      apply blast
+    using hb(3)
+      apply blast
+     apply (rule Strict)
+  proof
+    assume "kf_pos_turned_on opt"
+    thus "heap_knownfolded_rel_pos Pr FieldTr (get_nm_total_full \<omega>') hb"
+      using Strict PosImpliesStrict heap_knownfolded_rel_imp_pos
+      by simp
+  qed
+qed
 
 
 definition zero_knownfolded_mask where
